---
mathjax: true
---

{% include mathjax.html %}

## 1 以下の等式を証明せよ
$$ \sum_{i=1}^n (x_i - \bar x) = 0 $$

----

<div> $$ \begin{eqnarray*}
\sum_{i=1}^n (x_i - \bar x) &=& \sum_{i=1}^n x_i - n \bar x \\
&=& n \bar x - n \bar x = 0
\end{eqnarray*} $$ </div>

## 2 以下の等式を証明せよ
$$ \sum_{i=1}^n (x_i - \bar x)(y_i - \bar y) = \sum_{i=1}^n x_i y_i - n \bar x \bar y $$

----

<div> $$ \begin{eqnarray*}
\sum_{i=1}^n (x_i - \bar x)(y_i - \bar y)
&=& \sum_{i=1}^n x_i y_i + n \bar x \bar y - \bar x \sum_{i=1}^n (y_i - \bar y) - \bar y \sum_{i=1}^n (x_i - \bar x) \\
&=& \sum_{i=1}^n x_i y_i + n \bar x \bar y
\end{eqnarray*} $$ </div>

## 3 以下の等式を証明せよ
$$ \sum_{i=1}^n e_i = 0 $$

----

<div> $$ \begin{eqnarray*}
\sum_{i=1}^n e_i
&=& \sum_{i=1}^n (y_i - \hat y_i) \\
&=& 
\end{eqnarray*} $$ </div>
